

# Combinatorics of Schwinger Energy Hamiltonian Coefficients

So we have the following Hamiltonian

$$H_E = \sum_{i=0}^{N-2} \left( \frac{\theta}{2\pi} + \sum_{j=0}^i \frac{Z_j + (-1)^j}{2} \right)^2$$

First, we can divide out the common  $\left(\frac{1}{2}\right)^2$

$$H_E = \frac{1}{4} \sum_{i=0}^{N-2} \left( \frac{\theta}{\pi} + \sum_{j=0}^i Z_j + (-1)^j \right)^2$$

and we want to extract its coefficients. In order to do so, let's leverage some notational abstraction:

$$f(i) = \frac{\theta}{\pi} + \sum_{j=0}^i (-1)^j$$

Which we can reduce further using the following fact

$$\sum_{j=0}^i (-1)^j = ((i+1) \bmod 2)$$

making

$$f(i) = \frac{\theta}{\pi} + ((i+1) \bmod 2)$$

Plugging this all back into  $H_E$  we get

$$H_E = \frac{1}{4} \sum_{i=0}^{N-2} \left( f(i) + \sum_{j=0}^i Z_j \right)^2$$

Now, we can multiply the square out!

$$\begin{aligned}
H_E &= \frac{1}{4} \sum_{i=0}^{N-2} \left( f(i) + \sum_{j=0}^i Z_j \right)^2 \\
&= \frac{1}{4} \sum_{i=0}^{N-2} \left( f(i) + \sum_{j=0}^i Z_j \right) \left( f(i) + \sum_{k=0}^i Z_k \right) \\
&= \frac{1}{4} \sum_{i=0}^{N-2} \left( f(i)^2 + \sum_{j=0}^i \sum_{k=0}^i Z_j Z_k + 2f(i) \sum_{j=0}^i Z_j \right)
\end{aligned}$$

Great! Now we have our term separated into three more easily malleable terms.

## Identity

$$\begin{aligned}
\frac{1}{4} \sum_{i=0}^{N-2} f(i)^2 &= \frac{1}{4} \sum_{i=0}^{N-2} \left( \frac{\theta}{\pi} + ((i+1) \bmod 2) \right)^2 \\
&= \frac{1}{4} \sum_{i=0}^{N-2} \left( \frac{\theta}{\pi} \right)^2 + ((i+1) \bmod 2)^2 + 2 \frac{\theta}{\pi} ((i+1) \bmod 2) \\
&\text{Since } ((i+1) \bmod 2) \text{ can only be 0 or 1} \\
&= \frac{1}{4} \sum_{i=0}^{N-2} \left( \frac{\theta}{\pi} \right)^2 + ((i+1) \bmod 2) + 2 \frac{\theta}{\pi} ((i+1) \bmod 2) \\
&= \frac{1}{4} \sum_{i=0}^{N-2} \left( \frac{\theta}{\pi} \right)^2 + \left( 1 + 2 \frac{\theta}{\pi} \right) ((i+1) \bmod 2) \\
&= \frac{N-1}{4} \left( \frac{\theta}{\pi} \right)^2 + \frac{1}{4} \left\lceil \frac{N-1}{2} \right\rceil \left( 1 + 2 \frac{\theta}{\pi} \right)
\end{aligned}$$

## Two-Qubit

For the two-qubit coefficients we know that if  $j = k$  then  $Z_j Z_k = I$

$$\begin{aligned}
\frac{1}{4} \sum_{i=0}^{N-2} \sum_{j=0}^i \sum_{k=0}^i Z_j Z_k &= \frac{1}{4} \sum_{i=0}^{N-2} \sum_{j=0}^i \sum_{k=0}^i Z_j Z_k \\
&= \frac{1}{4} \frac{N(N-1)}{2} + \frac{1}{4} \sum_{i=0}^{N-2} \sum_{j=0}^i \sum_{k=0}^{j-1} 2 \cdot Z_j Z_k \\
&= \frac{N(N-1)}{8} + \frac{1}{2} \sum_{j=0}^{N-2} \sum_{k=0}^{j-1} (N-j-1) Z_j Z_k
\end{aligned}$$

## Single-Qubit

Finally we have the single-qubit coefficients

$$\begin{aligned}\frac{1}{4} \cdot 2 \sum_{i=0}^{N-2} f(i) \sum_{j=0}^i Z_j &= \frac{1}{2} \sum_{j=0}^{N-2} \sum_{i=j}^{N-2} f(i) Z_j \\ &= \frac{1}{2} \sum_{j=0}^{N-2} \sum_{i=j}^{N-2} \left( \frac{\theta}{\pi} + ((i+1) \bmod 2) \right) Z_j\end{aligned}$$

This term itself splits into two parts

$$\frac{\theta}{2\pi} \sum_{j=0}^{N-2} \sum_{i=j}^{N-2} Z_j = \sum_{j=0}^{N-2} \frac{\theta}{2\pi} (N-j-1) Z_j$$

and

$$\frac{1}{2} \sum_{j=0}^{N-2} \sum_{i=j}^{N-2} ((i+1) \bmod 2) Z_j = \sum_{j=0}^{N-2} \frac{1}{2} \left( \left\lceil \frac{N-j-1}{2} \right\rceil - ((j \cdot N) \bmod 2) \right) Z_j$$

Thus

$$\begin{aligned}& \frac{1}{2} \sum_{j=0}^{N-2} \sum_{i=j}^{N-2} \left( \frac{\theta}{\pi} + ((i+1) \bmod 2) \right) Z_j \\ &= \frac{1}{2} \sum_{j=0}^{N-2} \left( \frac{\theta}{\pi} (N-j-1) + \left\lceil \frac{N-j-1}{2} \right\rceil + ((j \cdot N) \bmod 2) \right) Z_j\end{aligned}$$

With the dust settled we have

## Identity

$$\frac{1}{4} \left( (N-1) \left( \frac{\theta}{\pi} \right)^2 + \left\lceil \frac{N-1}{2} \right\rceil \left( 1 + 2 \frac{\theta}{\pi} \right) + \frac{N(N-1)}{2} \right)$$

## Multi Qubit

$$\frac{1}{2} \sum_{j=0}^{N-2} \sum_{k=0}^{j-1} (N-j-1) Z_j Z_k$$

## Single Qubit

$$\frac{1}{2} \sum_{j=0}^{N-2} \left( \frac{\theta}{\pi} (N-j-1) + \left\lceil \frac{N-j-1}{2} \right\rceil - ((j \cdot N) \bmod 2) \right) Z_j$$

$$H_E = \frac{g^2 a}{2} \sum_{i=0}^{N-2} \left( \frac{\theta}{2\pi} + \sum_{j=0}^i \frac{Z_j + (-1)^j}{2} \right)^2$$

$$H_M = \frac{m}{2} \sum_{i=0}^{N-1} (-1)^i Z_i$$

$$H_I = \frac{1}{4a} \sum_{i=0}^{N-2} X_i X_{i+1} + Y_i Y_{i+1}$$